feat: Check valid materials less

AwsCryptographicMaterialProviders/dafny/AwsCryptographicMaterialProviders/src/CMM.dfy
@@ -12,49 +12,65 @@ module {:options "/functionSyntax:4" } CMM {
   trait {:termination false} VerifiableInterface
     extends Types.ICryptographicMaterialsManager
   {
-    method GetEncryptionMaterials'(input: Types.GetEncryptionMaterialsInput)
-      returns (output: Result<Types.GetEncryptionMaterialsOutput, Types.Error>)
-      requires ValidState()
-      modifies Modifies - {History}
-      // Dafny will skip type parameters when generating a default decreases clause.
-      decreases Modifies - {History}
-      ensures ValidState()
-      ensures GetEncryptionMaterialsEnsuresPublicly(input, output)
-      ensures unchanged(History)
-      ensures output.Success?
-              ==>
-                && Materials.EncryptionMaterialsHasPlaintextDataKey(output.value.encryptionMaterials)
-      ensures output.Success?
-              ==>
-                && RequiredEncryptionContextKeys?(input.requiredEncryptionContextKeys, output.value.encryptionMaterials)
 
-    method DecryptMaterials'(input: Types.DecryptMaterialsInput)
-      returns (output: Result<Types.DecryptMaterialsOutput, Types.Error>)
-      requires ValidState()
-      modifies Modifies - {History}
-      // Dafny will skip type parameters when generating a default decreases clause.
-      decreases Modifies - {History}
-      ensures ValidState()
-      ensures DecryptMaterialsEnsuresPublicly(input, output)
-      ensures unchanged(History)
-      ensures output.Success?
-              ==>
-                && Materials.DecryptionMaterialsWithPlaintextDataKey(output.value.decryptionMaterials)
-      //= aws-encryption-sdk-specification/framework/cmm-interface.md#decrypt-materials
-      //# The CMM MUST validate the [Encryption Context](structures.md#encryption-context)
-      //# by comparing it to the customer supplied [Reproduced Encryption Context](structures.md#encryption-context)
-      //# in [decrypt materials request](#decrypt-materials-request).
-      //# For every key that exists in both [Reproduced Encryption Context](structures.md#encryption-context)
-      //# and [Encryption Context](structures.md#encryption-context),
-      //# the values MUST be equal or the operation MUST fail.
+    ghost predicate GetEncryptionMaterialsEnsuresPublicly(input: Types.GetEncryptionMaterialsInput, output: Result<Types.GetEncryptionMaterialsOutput, Types.Error>)
+      : (outcome: bool)
       ensures
-        && (output.Success? ==> ReproducedEncryptionContext?(input))
-        && (!ReproducedEncryptionContext?(input) ==> output.Failure?)
-      //= aws-encryption-sdk-specification/framework/cmm-interface.md#decrypt-materials
-      //# - All key-value pairs that exist in [Reproduced Encryption Context](structures.md#encryption-context)
-      //# but do not exist in encryption context on the [decrypt materials request](#decrypt-materials-request)
-      //# SHOULD be appended to the decryption materials.
-      ensures output.Success? ==> EncryptionContextComplete(input, output.value.decryptionMaterials)
+        outcome ==>
+          output.Success?
+          ==>
+            // if the output materials are valid then they contain the required fields
+            //= aws-encryption-sdk-specification/framework/cmm-interface.md#get-encryption-materials
+            //= type=implication
+            //# The encryption materials returned MUST include the following:
+
+            // See EncryptionMaterialsHasPlaintextDataKey for details
+            //= aws-encryption-sdk-specification/framework/cmm-interface.md#get-encryption-materials
+            //= type=implication
+            //# The CMM MUST ensure that the encryption materials returned are valid.
+            //# - The encryption materials returned MUST follow the specification for [encryption-materials](structures.md#encryption-materials).
+            //# - The value of the plaintext data key MUST be non-NULL.
+            //# - The plaintext data key length MUST be equal to the [key derivation input length](algorithm-suites.md#key-derivation-input-length).
+            //# - The encrypted data keys list MUST contain at least one encrypted data key.
+            //# - If the algorithm suite contains a signing algorithm, the encryption materials returned MUST include the generated signing key.
+            //# - For every key in [Required Encryption Context Keys](structures.md#required-encryption-context-keys)
+            //#   there MUST be a matching key in the [Encryption Context](structures.md#encryption-context-1).
+            && Materials.EncryptionMaterialsHasPlaintextDataKey(output.value.encryptionMaterials)
+               //= aws-encryption-sdk-specification/framework/cmm-interface.md#get-encryption-materials
+               //= type=implication
+               //# - The [Required Encryption Context Keys](structures.md#required-encryption-context-keys) MUST be
+               //#   a super set of the Required Encryption Context Keys in the [encryption materials request](#encryption-materials-request).
+            && RequiredEncryptionContextKeys?(input.requiredEncryptionContextKeys, output.value.encryptionMaterials)
+
+    ghost predicate DecryptMaterialsEnsuresPublicly(input: Types.DecryptMaterialsInput, output: Result<Types.DecryptMaterialsOutput, Types.Error>)
+      : (outcome: bool)
+      ensures
+        outcome ==>
+          // if the output materials are valid then they contain the required fields
+          //= aws-encryption-sdk-specification/framework/cmm-interface.md#decrypt-materials
+          //= type=implication
+          //# The decryption materials returned MUST include the following:
+          && (output.Success?
+              //= aws-encryption-sdk-specification/framework/cmm-interface.md#decrypt-materials
+              //= type=implication
+              //# The CMM MUST ensure that the decryption materials returned are valid.
+              //# - The decryption materials returned MUST follow the specification for [decryption-materials](structures.md#decryption-materials).
+              //# - The value of the plaintext data key MUST be non-NULL.
+              ==> Materials.DecryptionMaterialsWithPlaintextDataKey(output.value.decryptionMaterials))
+             //= aws-encryption-sdk-specification/framework/cmm-interface.md#decrypt-materials
+             //# The CMM MUST validate the [Encryption Context](structures.md#encryption-context)
+             //# by comparing it to the customer supplied [Reproduced Encryption Context](structures.md#encryption-context)
+             //# in [decrypt materials request](#decrypt-materials-request).
+             //# For every key that exists in both [Reproduced Encryption Context](structures.md#encryption-context)
+             //# and [Encryption Context](structures.md#encryption-context),
+             //# the values MUST be equal or the operation MUST fail.
+          && (output.Success? ==> ReproducedEncryptionContext?(input))
+          && (!ReproducedEncryptionContext?(input) ==> output.Failure?)
+             //= aws-encryption-sdk-specification/framework/cmm-interface.md#decrypt-materials
+             //# - All key-value pairs that exist in [Reproduced Encryption Context](structures.md#encryption-context)
+             //# but do not exist in encryption context on the [decrypt materials request](#decrypt-materials-request)
+             //# SHOULD be appended to the decryption materials.
+          && (output.Success? ==> EncryptionContextComplete(input, output.value.decryptionMaterials))
   }
 
   predicate RequiredEncryptionContextKeys?(requiredEncryptionContextKeys: Option<Types.EncryptionContextKeys>, encryptionMaterials: Types.EncryptionMaterials) {
@@ -64,7 +80,7 @@ module {:options "/functionSyntax:4" } CMM {
 
   predicate EncryptionContextComplete(input: Types.DecryptMaterialsInput, decryptionMaterials: Types.DecryptionMaterials) {
     var reproducedEncryptionContext := input.reproducedEncryptionContext.UnwrapOr(map[]);
-    forall k <- reproducedEncryptionContext.Keys
+    forall k <- reproducedEncryptionContext
       ::
         && k in decryptionMaterials.encryptionContext
         && decryptionMaterials.encryptionContext[k] == reproducedEncryptionContext[k]
@@ -72,7 +88,7 @@ module {:options "/functionSyntax:4" } CMM {
 
   predicate ReproducedEncryptionContext?(input: Types.DecryptMaterialsInput) {
     var reproducedEncryptionContext := input.reproducedEncryptionContext.UnwrapOr(map[]);
-    forall k <- reproducedEncryptionContext.Keys
+    forall k <- reproducedEncryptionContext
            | k in input.encryptionContext
       :: input.encryptionContext[k] == reproducedEncryptionContext[k]
   }
