AwsCryptographicMaterialProviders/dafny/AwsCryptographicMaterialProviders/src/Keyrings/MultiKeyring.dfy
@@ -95,7 +95,28 @@ module MultiKeyring {
     }
 
 
-    predicate OnEncryptEnsuresPublicly(input: Types.OnEncryptInput, output: Result<Types.OnEncryptOutput, Types.Error>) {true}
+    predicate OnEncryptEnsuresPublicly (
+      input: Types.OnEncryptInput ,
+      output: Result<Types.OnEncryptOutput, Types.Error> )
+      : (outcome: bool)
+      ensures
+        outcome ==>
+          output.Success?
+          ==>
+            && Materials.EncryptionMaterialsHasPlaintextDataKey(output.value.materials)
+            && Materials.ValidEncryptionMaterialsTransition(
+                 input.materials,
+                 output.value.materials
+               )
+    {
+      output.Success?
+      ==>
+        && Materials.EncryptionMaterialsHasPlaintextDataKey(output.value.materials)
+        && Materials.ValidEncryptionMaterialsTransition(
+             input.materials,
+             output.value.materials
+           )
+    }
     //= aws-encryption-sdk-specification/framework/multi-keyring.md#generator-keyring
     //= type=implication
     //# This keyring MUST implement the [Generate Data Key](keyring-
