AwsCryptographicMaterialProviders/dafny/AwsCryptographicMaterialProviders/test/Keyrings/TestMultiKeyring.dfy
@@ -350,8 +350,46 @@ module TestMultiKeyring {
       && History in Modifies
     }
 
-    predicate OnEncryptEnsuresPublicly(input: Types.OnEncryptInput, output: Result<Types.OnEncryptOutput, Types.Error>) {true}
-    predicate OnDecryptEnsuresPublicly(input: Types.OnDecryptInput, output: Result<Types.OnDecryptOutput, Types.Error>){true}
+    predicate OnEncryptEnsuresPublicly (
+      input: Types.OnEncryptInput ,
+      output: Result<Types.OnEncryptOutput, Types.Error> )
+      : (outcome: bool)
+      ensures
+        outcome ==>
+          output.Success?
+          ==>
+            && Materials.EncryptionMaterialsHasPlaintextDataKey(output.value.materials)
+            && Materials.ValidEncryptionMaterialsTransition(
+                 input.materials,
+                 output.value.materials
+               )
+    {
+      output.Success?
+      ==>
+        && Materials.EncryptionMaterialsHasPlaintextDataKey(output.value.materials)
+        && Materials.ValidEncryptionMaterialsTransition(
+             input.materials,
+             output.value.materials
+           )
+    }
+    predicate OnDecryptEnsuresPublicly ( input: Types.OnDecryptInput , output: Result<Types.OnDecryptOutput, Types.Error> )
+      : (outcome: bool)
+      ensures
+        outcome ==>
+          output.Success?
+          ==>
+            && Materials.DecryptionMaterialsTransitionIsValid(
+              input.materials,
+              output.value.materials
+            )
+    {
+      output.Success?
+      ==>
+        && Materials.DecryptionMaterialsTransitionIsValid(
+          input.materials,
+          output.value.materials
+        )
+    }
 
     constructor(
       encryptionMaterials: Option<Types.EncryptionMaterials>,
@@ -410,8 +448,46 @@ module TestMultiKeyring {
       && History in Modifies
     }
 
-    predicate OnEncryptEnsuresPublicly(input: Types.OnEncryptInput, output: Result<Types.OnEncryptOutput, Types.Error>) {true}
-    predicate OnDecryptEnsuresPublicly(input: Types.OnDecryptInput, output: Result<Types.OnDecryptOutput, Types.Error>){true}
+    predicate OnEncryptEnsuresPublicly (
+      input: Types.OnEncryptInput ,
+      output: Result<Types.OnEncryptOutput, Types.Error> )
+      : (outcome: bool)
+      ensures
+        outcome ==>
+          output.Success?
+          ==>
+            && Materials.EncryptionMaterialsHasPlaintextDataKey(output.value.materials)
+            && Materials.ValidEncryptionMaterialsTransition(
+                 input.materials,
+                 output.value.materials
+               )
+    {
+      output.Success?
+      ==>
+        && Materials.EncryptionMaterialsHasPlaintextDataKey(output.value.materials)
+        && Materials.ValidEncryptionMaterialsTransition(
+             input.materials,
+             output.value.materials
+           )
+    }
+    predicate OnDecryptEnsuresPublicly ( input: Types.OnDecryptInput , output: Result<Types.OnDecryptOutput, Types.Error> )
+      : (outcome: bool)
+      ensures
+        outcome ==>
+          output.Success?
+          ==>
+            && Materials.DecryptionMaterialsTransitionIsValid(
+              input.materials,
+              output.value.materials
+            )
+    {
+      output.Success?
+      ==>
+        && Materials.DecryptionMaterialsTransitionIsValid(
+          input.materials,
+          output.value.materials
+        )
+    }
 
     constructor()
       ensures ValidState() && fresh(History) && fresh(Modifies)
